Some progress
Signed-off-by: zeramorphic <zeramorphic@proton.me>

ConNF/Counting/Spec.lean
@@ -108,34 +108,73 @@ theorem inflexible_of_mem_dom_nearLitterCondInflexRel
   obtain ⟨c, P, t, hA, ht, _⟩ := h
   exact ⟨P, t, hA, ht⟩
 
-theorem nearLitterCondRel_dom_disjoint
-     {S : Support β} {A : β ↝ ⊥} :
+theorem nearLitterCondRel_dom_disjoint {S : Support β} {A : β ↝ ⊥} :
     Disjoint (nearLitterCondRelFlex S A).dom (nearLitterCondRelInflex S A).dom := by
   rw [Set.disjoint_iff_forall_ne]
   rintro N hN₁ _ hN₂ rfl
   exact flexible_of_mem_dom_nearLitterCondFlexRel hN₁
     (inflexible_of_mem_dom_nearLitterCondInflexRel hN₂)
 
-theorem nearLitterCondRel_coinjective
-     {S : Support β} {A : β ↝ ⊥} :
+theorem nearLitterCondRel_coinjective (S : Support β) (A : β ↝ ⊥) :
     (nearLitterCondRel S A).Coinjective :=
   Rel.sup_coinjective
     nearLitterCondRelFlex_coinjective
     nearLitterCondRelInflex_coinjective
     nearLitterCondRel_dom_disjoint
 
-def Support.spec  (S : Support β) : Spec β where
+theorem nearLitterCondRel_cosurjective (S : Support β) (A : β ↝ ⊥) :
+    (nearLitterCondRel S A).Cosurjective := by
+  constructor
+  intro N
+  obtain (⟨P, t, hA, ht⟩ | hN) := inflexible_cases A Nᴸ
+  · exact ⟨_, Or.inr ⟨P, t, hA, ht, rfl⟩⟩
+  · exact ⟨_, Or.inl ⟨hN, rfl⟩⟩
+
+def Support.spec (S : Support β) : Spec β where
   atoms A := (S ⇘. A)ᴬ.image
     (λ a ↦ ⟨{i | (S ⇘. A)ᴬ.rel i a}, {i | ∃ N, (S ⇘. A)ᴺ.rel i N ∧ a ∈ Nᴬ}⟩)
   nearLitters A := (S ⇘. A)ᴺ.comp
-    (nearLitterCondRel S A) nearLitterCondRel_coinjective
+    (nearLitterCondRel S A) (nearLitterCondRel_coinjective S A)
 
-def convAtoms  (S T : Support β) (A : β ↝ ⊥) : Rel Atom Atom :=
+theorem Support.spec_atoms_dom (S : Support β) (A : β ↝ ⊥) :
+    (S.specᴬ A).rel.dom = (S ⇘. A)ᴬ.rel.dom := by
+  ext i
+  constructor
+  · rintro ⟨c, a, h, _⟩
+    exact ⟨a, h⟩
+  · rintro ⟨a, h⟩
+    exact ⟨_, a, h, rfl⟩
+
+theorem Support.spec_nearLitters_dom (S : Support β) (A : β ↝ ⊥) :
+    (S.specᴺ A).rel.dom = (S ⇘. A)ᴺ.rel.dom := by
+  ext i
+  constructor
+  · rintro ⟨c, a, h, _⟩
+    exact ⟨a, h⟩
+  · rintro ⟨N, h⟩
+    obtain ⟨c, hc⟩ := (nearLitterCondRel_cosurjective S A).cosurjective N
+    exact ⟨c, N, h, hc⟩
+
+def convAtoms (S T : Support β) (A : β ↝ ⊥) : Rel Atom Atom :=
   (S ⇘. A)ᴬ.rel.inv.comp (T ⇘. A)ᴬ.rel
 
 def convNearLitters (S T : Support β) (A : β ↝ ⊥) :
     Rel NearLitter NearLitter :=
   (S ⇘. A)ᴺ.rel.inv.comp (T ⇘. A)ᴺ.rel
+
+@[simp]
+theorem convAtoms_inv (S T : Support β) (A : β ↝ ⊥) :
+    (convAtoms S T A).inv = convAtoms T S A := by
+  ext a b
+  simp only [Rel.inv, flip, convAtoms, Rel.comp]
+  tauto
+
+@[simp]
+theorem convNearLitters_inv (S T : Support β) (A : β ↝ ⊥) :
+    (convNearLitters S T A).inv = convNearLitters T S A := by
+  ext a b
+  simp only [Rel.inv, flip, convNearLitters, Rel.comp]
+  tauto
 
 def atomMemRel (S : Support β) (A : β ↝ ⊥) : Rel κ κ :=
   (S ⇘. A)ᴺ.rel.comp (Rel.comp (λ N a ↦ a ∈ Nᴬ) (S ⇘. A)ᴬ.rel.inv)
@@ -147,8 +186,8 @@ structure SameSpec (S T : Support β) : Prop where
 (atomMemRel_eq : ∀ A, atomMemRel S A = atomMemRel T A)
 (inflexible_iff : ∀ {A N₁ N₂}, convNearLitters S T A N₁ N₂ →
   ∀ P : InflexiblePath β, ∀ t : Tangle P.δ, A = P.A ↘ P.hε ↘. →
-  (∃ ρ : AllPerm P.δ, N₁ᴸ = fuzz P.hδε (ρ • t)) ↔
-  (∃ ρ : AllPerm P.δ, N₂ᴸ = fuzz P.hδε (ρ • t)))
+  ((∃ ρ : AllPerm P.δ, N₁ᴸ = fuzz P.hδε (ρ • t)) ↔
+  (∃ ρ : AllPerm P.δ, N₂ᴸ = fuzz P.hδε (ρ • t))))
 (litter_eq_iff_of_flexible : ∀ {A N₁ N₂ N₃ N₄},
   convNearLitters S T A N₁ N₂ → convNearLitters S T A N₃ N₄ →
   ¬Inflexible A N₁ᴸ → ¬Inflexible A N₂ᴸ → (N₁ᴸ = N₃ᴸ ↔ N₂ᴸ = N₄ᴸ))
@@ -165,13 +204,85 @@ structure SameSpec (S T : Support β) : Prop where
     convNearLitters (S ⇘ (P.A ↘ P.hδ)) (T ⇘ (P.A ↘ P.hδ)) B ⊓ (λ a _ ↦ a ∈ (t.support ⇘. B)ᴺ) ≤
       (λ N₁ N₂ ↦ N₂ = ρᵁ ⇘. B • N₁))
 
+/-- A variant of `SameSpec` in which most equalities have been turned into one-directional
+implications. It can sometimes be easier to prove this in generality than to prove `SameSpec`
+directly. -/
+structure SameSpecLE (S T : Support β) : Prop where
+(atoms_dom_subset : ∀ A, (S ⇘. A)ᴬ.rel.dom ⊆ (T ⇘. A)ᴬ.rel.dom)
+(nearLitters_dom_subset : ∀ A, (S ⇘. A)ᴺ.rel.dom ⊆ (T ⇘. A)ᴺ.rel.dom)
+(convAtoms_injective : ∀ A, (convAtoms S T A).Injective)
+(atomMemRel_le : ∀ A, atomMemRel S A ≤ atomMemRel T A)
+(inflexible_of_inflexible : ∀ {A N₁ N₂}, convNearLitters S T A N₁ N₂ →
+  ∀ P : InflexiblePath β, ∀ t : Tangle P.δ, A = P.A ↘ P.hε ↘. →
+  N₁ᴸ = fuzz P.hδε t → ∃ ρ : AllPerm P.δ, N₂ᴸ = fuzz P.hδε (ρ • t))
+(litter_eq_of_flexible : ∀ {A N₁ N₂ N₃ N₄},
+  convNearLitters S T A N₁ N₂ → convNearLitters S T A N₃ N₄ →
+  ¬Inflexible A N₁ᴸ → ¬Inflexible A N₂ᴸ → (N₁ᴸ = N₃ᴸ → N₂ᴸ = N₄ᴸ))
+(convAtoms_of_inflexible : ∀ A, ∀ N₁ N₂ : NearLitter,
+  ∀ P : InflexiblePath β, ∀ t : Tangle P.δ, ∀ ρ : AllPerm P.δ,
+  A = P.A ↘ P.hε ↘. ∧ N₁ᴸ = fuzz P.hδε t → N₂ᴸ = fuzz P.hδε (ρ • t) →
+  ∀ B : P.δ ↝ ⊥,
+    convAtoms (S ⇘ (P.A ↘ P.hδ)) (T ⇘ (P.A ↘ P.hδ)) B ⊓ (λ a _ ↦ a ∈ (t.support ⇘. B)ᴬ) ≤
+      (λ a b ↦ b = ρᵁ ⇘. B • a))
+(convNearLitters_of_inflexible : ∀ A, ∀ N₁ N₂ : NearLitter,
+  ∀ P : InflexiblePath β, ∀ t : Tangle P.δ, ∀ ρ : AllPerm P.δ,
+  A = P.A ↘ P.hε ↘. ∧ N₁ᴸ = fuzz P.hδε t → N₂ᴸ = fuzz P.hδε (ρ • t) →
+  ∀ B : P.δ ↝ ⊥,
+    convNearLitters (S ⇘ (P.A ↘ P.hδ)) (T ⇘ (P.A ↘ P.hδ)) B ⊓ (λ a _ ↦ a ∈ (t.support ⇘. B)ᴺ) ≤
+      (λ N₁ N₂ ↦ N₂ = ρᵁ ⇘. B • N₁))
+
+theorem sameSpec_antisymm {S T : Support β} (h₁ : SameSpecLE S T) (h₂ : SameSpecLE T S) :
+    SameSpec S T where
+  atoms_dom_eq A := subset_antisymm (h₁.atoms_dom_subset A) (h₂.atoms_dom_subset A)
+  nearLitters_dom_eq A := subset_antisymm (h₁.nearLitters_dom_subset A) (h₂.nearLitters_dom_subset A)
+  convAtoms_oneOne A := ⟨h₁.convAtoms_injective A,
+    Rel.inv_injective_iff.mp (convAtoms_inv S T A ▸ h₂.convAtoms_injective A)⟩
+  atomMemRel_eq A := le_antisymm (h₁.atomMemRel_le A) (h₂.atomMemRel_le A)
+  inflexible_iff h P t hA := by
+    constructor
+    · rintro ⟨ρ, ht⟩
+      obtain ⟨ρ', ht'⟩ := h₁.inflexible_of_inflexible h P (ρ • t) hA ht
+      use ρ' * ρ
+      rw [ht', mul_smul]
+    · rintro ⟨ρ, ht⟩
+      obtain ⟨ρ', ht'⟩ := h₂.inflexible_of_inflexible (convNearLitters_inv T S _ ▸ h) P (ρ • t) hA ht
+      use ρ' * ρ
+      rw [ht', mul_smul]
+  litter_eq_iff_of_flexible hN₁ hN₂ hN₁' hN₂' := ⟨h₁.litter_eq_of_flexible hN₁ hN₂ hN₁' hN₂',
+    h₂.litter_eq_of_flexible
+      (convNearLitters_inv S T _ ▸ hN₁) (convNearLitters_inv S T _ ▸ hN₂) hN₂' hN₁'⟩
+  convAtoms_of_inflexible := h₁.convAtoms_of_inflexible
+  convNearLitters_of_inflexible := h₁.convNearLitters_of_inflexible
+
 namespace Support
 
 variable {S T : Support β}
 
+theorem atoms_dom_subset_of_spec_eq_spec (h : S.spec = T.spec) (A : β ↝ ⊥) :
+    (S ⇘. A)ᴬ.rel.dom ⊆ (T ⇘. A)ᴬ.rel.dom := by
+  rw [← spec_atoms_dom, ← spec_atoms_dom, h]
+
+theorem nearLitters_dom_subset_of_spec_eq_spec (h : S.spec = T.spec) (A : β ↝ ⊥) :
+    (S ⇘. A)ᴺ.rel.dom ⊆ (T ⇘. A)ᴺ.rel.dom := by
+  rw [← spec_nearLitters_dom, ← spec_nearLitters_dom, h]
+
+theorem sameSpecLe_of_spec_eq_spec (h : S.spec = T.spec) :
+    SameSpecLE S T where
+  atoms_dom_subset := atoms_dom_subset_of_spec_eq_spec h
+  nearLitters_dom_subset := nearLitters_dom_subset_of_spec_eq_spec h
+  convAtoms_injective := sorry
+  atomMemRel_le := sorry
+  inflexible_of_inflexible := sorry
+  litter_eq_of_flexible := sorry
+  convAtoms_of_inflexible := sorry
+  convNearLitters_of_inflexible := sorry
+
 theorem spec_eq_spec_iff (S T : Support β) :
     S.spec = T.spec ↔ SameSpec S T := by
-  sorry
+  constructor
+  · intro h
+    exact sameSpec_antisymm (sameSpecLe_of_spec_eq_spec h) (sameSpecLe_of_spec_eq_spec h.symm)
+  · sorry
 
 end Support
 
